\documentclass[12pt, letterpaper]{article}
\usepackage{graphicx}
\usepackage{amsmath}
\usepackage{amssymb}
\usepackage{float}
\graphicspath{{images/}}
\title{Closed Form formula sor simple linear regression}
\author{Evert Jan Karman}
\date{January 1900}
\begin{document}
\maketitle

Documenting the closed form formula for simple linear regression

\section{The gradient formula for RSS}
\[
\nabla RSS(w_0,w_1) = \left( \frac{\partial RSS}{\partial w_0}, \frac{\partial RSS}{\partial w_1} \right)
\]
Where
\[
\frac{\partial RSS}{\partial w_0} = -2 \cdot \sum_{i=0}^{N-1} \left( y_i - (w_0 + w_1 x_i) \right)
\]
And
\[
\frac{\partial RSS}{\partial w_1} = -2 \cdot \sum_{i=0}^{N-1} \left( (y_i - (w_0 + w_1 x_i)) \cdot x_i \right)
\]

\section{Solving for gradient eq zero}
When we solve for gradient = zero, we get
\[
w_0 \cdot N = \sum_{i=0}^{N-1} y_i - w_1 \cdot \sum_{i=0}^{N-1} x_i
\]
and
\[
w_0 \cdot \sum_{i=0}^{N-1} x_i = \sum_{i=0}^{N-1} y_i \cdot x_i - w_1 \cdot \sum_{i=0}^{N-1} x_i^2
\]
We are looking at a system of two equations:
\begin{align*}
w_0 \cdot N &= A - w_1 \cdot B \\
w_0 \cdot B &= C - w_1 \cdot D
\end{align*}

With A, B, C, D expressions not dependent on $w_0$ or $w_1$
\begin{align*}
A &= \sum_{i=0}^{N-1} y_i \\
B &= \sum_{i=0}^{N-1} x_i \\
C &= \sum_{i=0}^{N-1} x_i \cdot y_i \\
D &= \sum_{i=0}^{N-1} x_i^2
\end{align*}

So that
\[
w_1 = \frac{C - \frac{A \cdot B}{N}}{D - \frac{B \cdot B}{N}}
\]
And then
\[
w_0 = \frac{A}{N} - w_1 \cdot \frac{B}{N}
\]

\end{document}
